Make implicit squash arguments work again.

pulse/src/checker/Pulse.Checker.ST.fst
@@ -23,6 +23,7 @@ open Pulse.Checker.Base
 
 module T = FStar.Tactics.V2
 module RT = FStar.Reflection.Typing
+module R = FStar.Reflection.V2
 module RU = Pulse.RuntimeUtils
 module P = Pulse.Syntax.Printer
 module Prover = Pulse.Checker.Prover
@@ -30,6 +31,35 @@ open Pulse.Show
 
 let should_allow_ambiguous (t:term) : T.Tac bool =
   Pulse.Reflection.Util.head_has_attr_string "Pulse.Lib.Core.allow_ambiguous" t
+
+// HACK: Instantiates implicits at the end with uvs
+// If we let instantiate_term_implicits_uvs instantiate these implicits,
+// then it will instantiate squash arguments with ().
+// The () will usually only type-check after running the prover,
+// however the prover requires a type-correct term.
+// Therefore we manually instantiate these implicits...
+let instantiate_term_implicits_uvs (g:env) (t:term)
+  : T.Tac (uvs:env { disjoint g uvs } & term & term) =
+  let (| uvs, t, ty |) = Pulse.Checker.Pure.instantiate_term_implicits_uvs g t false in
+  let rec add_implicits (uvs: env { disjoint g uvs }) (t ty:term)
+    : T.Tac (uvs:env { disjoint g uvs } & term & term) =
+    match inspect_ln_unascribe ty with
+    | R.Tv_Arrow b c ->
+      (match R.inspect_comp c with
+      | C_Total ty ->
+        let b = R.inspect_binder b in
+        if Q_Implicit? b.qual then
+          let x = fresh uvs in
+          let px = ppname_default, x in
+          let uvs = push_binding uvs x (fst px) b.sort in
+          assume disjoint g uvs;
+          let ty = open_term_nv ty px in
+          add_implicits uvs (pack_ln (R.Tv_App t (term_of_nvar px, b.qual))) ty
+        else
+          (| uvs, t, ty |)
+      | _ -> (| uvs, t, ty |))
+    | _ -> (| uvs, t, ty |) in
+  add_implicits uvs t ty
 
 let check
   (g0:env)
@@ -44,7 +74,7 @@ let check
   let post_hint: post_hint_opt g = post_hint in
   let range = t.range in
   let Tm_ST { t=e } = t.term in
-  let (| uvs, e, _ |) = Pulse.Checker.Pure.instantiate_term_implicits_uvs g e true in
+  let (| uvs, e, _ |) = instantiate_term_implicits_uvs g e in
   let g' : env = push_env g uvs in
   assert (g' `env_extends` g);
   let post_hint: post_hint_opt g' = post_hint in
